small bug fixes + some documentation

ml_sources/examples/reliable_communication/lib/sharding/sharding_code.ml
@@ -4,16 +4,16 @@ open Serialization_code
 open Mt_server_code
 open List_code
 
-(** Serializers *)
+(** Serializers **)
 
 let write_serializer (key_ser[@metavar]) (val_ser[@metavar]) =
   prod_serializer key_ser val_ser
-let read_serializer (key_ser[@metavar]) = key_ser
 let req_ser (key_ser[@metavar]) (val_ser[@metavar]) =
-  (sum_serializer (write_serializer key_ser val_ser) (read_serializer key_ser))
+  (sum_serializer (write_serializer key_ser val_ser) key_ser)
 let rep_ser (val_ser[@metavar]) =
   (sum_serializer (unit_serializer) (option_serializer val_ser))
 
+(** Server's behavior **)
 let client_request_handler_at_server data hash req =
   let k = (* Get the request's key k *)
     match req with
@@ -30,7 +30,7 @@ let client_request_handler_at_server data hash req =
   in
   let (rpc, lk) = p in (* Get the data corresponding to the shard assigned to k *)
   acquire lk;
-  let res = make_request rpc req in
+  let res = make_request rpc req in (* Redirect the request to that shard *)
   release lk;
   res
 
@@ -38,6 +38,7 @@ let start_server (key_ser[@metavar]) (val_ser[@metavar]) addr data hash () =
   run_server (rep_ser val_ser) (req_ser key_ser val_ser) addr
     (fun req -> client_request_handler_at_server data hash req)
 
+(** Shard's behavior **)
 let server_request_handler_at_shard db lk req =
   acquire lk;
   let res =
@@ -56,7 +57,10 @@ let start_shard (key_ser[@metavar]) (val_ser[@metavar]) addr db lk () =
   run_server (rep_ser val_ser) (req_ser key_ser val_ser) addr
     (fun req -> server_request_handler_at_shard db lk req)
 
-let init_server (key_ser[@metavar]) (val_ser[@metavar]) srv_addr addrs (hash : string -> int) =
+(** Initializes the server **)
+(* addrs contains couples of addresses linking the server to a shard *)
+(* hash has to return an integer smaller than the length of addrs, so that it can be used as an index *)
+let init_server (key_ser[@metavar]) (val_ser[@metavar]) srv_addr (addrs : (saddr * saddr) alist) (hash : string -> int) =
   let data = list_map (
                  fun p ->
                  let (srv, shard) = p in
@@ -65,11 +69,13 @@ let init_server (key_ser[@metavar]) (val_ser[@metavar]) srv_addr addrs (hash : s
                  (rpc, lk)) addrs in
   fork (start_server key_ser val_ser srv_addr data hash) ()
 
+(** Initializes a shard **)
 let init_shard (key_ser[@metavar]) (val_ser[@metavar]) addr =
   let db = ref (map_empty ()) in
   let lk = newlock () in
   fork (start_shard key_ser val_ser addr db lk) ()
 
+(** Initializes a client **)
 let init_client (key_ser[@metavar]) (val_ser[@metavar]) clt_addr srv_addr =
   let rpc = init_client_proxy (req_ser key_ser val_ser) (rep_ser val_ser) clt_addr srv_addr in
   let lk = newlock () in
